MPL/Specs.lean
@@ -65,7 +65,7 @@ theorem Zipper.atSuff_tail (l : List α) (h : hd::tl <:+ l): (Zipper.atSuff h).t
 
 end List
 
-theorem Specs.forIn_list {α : Type u} {β : Type} ⦃m : Type → Type v⦄ {ps : PredShape}
+theorem Specs.forIn_list {α : Type} {β : Type} ⦃m : Type → Type v⦄ {ps : PredShape}
   [Monad m] [LawfulMonad m] [WP m ps] [WPMonad m ps]
   {xs : List α} {init : β} {f : α → β → m (ForInStep β)}
   (inv : PostCond (β × List.Zipper xs) ps)
@@ -97,7 +97,7 @@ theorem Specs.forIn_list {α : Type u} {β : Type} ⦃m : Type → Type v⦄ {ps
 
 -- using the postcondition as a constant invariant:
 @[spec]
-theorem Specs.forIn_list_const_inv {α : Type u} {β : Type} ⦃m : Type → Type v⦄ {ps : PredShape}
+theorem Specs.forIn_list_const_inv {α : Type} {β : Type} ⦃m : Type → Type v⦄ {ps : PredShape}
   [Monad m] [LawfulMonad m] [WP m ps] [WPMonad m ps]
   {xs : List α} {init : β} {f : α → β → m (ForInStep β)}
   {inv : PostCond β ps}
@@ -108,7 +108,7 @@ theorem Specs.forIn_list_const_inv {α : Type u} {β : Type} ⦃m : Type → Typ
   ⦃inv.1 init⦄ forIn xs init f ⦃inv⦄ :=
     Specs.forIn_list (fun p => inv.1 p.1, inv.2) (fun b _ hd _ _ => step hd b)
 
-theorem Specs.foldlM_list {α : Type u} {β : Type} ⦃m : Type → Type v⦄ {ps : PredShape}
+theorem Specs.foldlM_list {α : Type} {β : Type} ⦃m : Type → Type v⦄ {ps : PredShape}
   [Monad m] [LawfulMonad m] [WP m ps] [WPMonad m ps]
   {xs : List α} {init : β} {f : β → α → m β}
   (inv : PostCond (β × List.Zipper xs) ps)
@@ -126,7 +126,7 @@ theorem Specs.foldlM_list {α : Type u} {β : Type} ⦃m : Type → Type v⦄ {p
 
 -- using the postcondition as a constant invariant:
 @[spec]
-theorem Specs.foldlM_list_const_inv {α : Type u} {β : Type} ⦃m : Type → Type v⦄ {ps : PredShape}
+theorem Specs.foldlM_list_const_inv {α : Type} {β : Type} ⦃m : Type → Type v⦄ {ps : PredShape}
   [Monad m] [LawfulMonad m] [WP m ps] [WPMonad m ps]
   {xs : List α} {init : β} {f : β → α → m β}
   {inv : PostCond β ps}
